src/Crypto/HKDF/HMAC.dfy
@@ -1,8 +1,8 @@
-include "../Digests.dfy"
+include "../KeyDerivationAlgorithms.dfy"
 include "../../StandardLibrary/StandardLibrary.dfy"
 
 module {:extern "HMAC"} HMAC {
-  import opened Digests
+  import opened KeyDerivationAlgorithms
   import opened StandardLibrary
   import opened UInt = StandardLibrary.UInt
 
